Attempt2/Connection.dfy
@@ -1,0 +1,883 @@
+module Connection {
+
+  import opened Circ
+  import opened Utils
+  import opened Entity
+  import opened Subcircuit
+  import opened Eval
+  import opened ConservedSubcircuit
+
+  opaque ghost predicate ConnectionValid(c: Circuit, e1: Entity, e2: Entity, connection: map<NP, NP>)
+    requires ScValid(c, e1.sc)
+    requires ScValid(c, e2.sc)
+  {
+    && (connection.Keys <= e2.finputs * AllINPs(c, e2.sc))
+    && (connection.Values <= e1.foutputs * AllONPs(c, e1.sc))
+    && SetsNoIntersection(connection.Keys, c.PortSource.Keys)
+  }
+
+  lemma ConnectionValuesInE1(c: Circuit, e1: Entity, e2: Entity, connection: map<NP, NP>)
+    requires ScValid(c, e1.sc)
+    requires ScValid(c, e2.sc)
+    requires ConnectionValid(c, e1, e2, connection)
+    ensures NPsInSc(e1.sc, connection.Values)
+  {
+    reveal ScValid();
+    reveal ConnectionValid();
+    reveal NPsInSc();
+  }
+
+  lemma ConnectionKeysInE2(c: Circuit, e1: Entity, e2: Entity, connection: map<NP, NP>)
+    requires ScValid(c, e1.sc)
+    requires ScValid(c, e2.sc)
+    requires ConnectionValid(c, e1, e2, connection)
+    ensures NPsInSc(e2.sc, connection.Keys)
+  {
+    reveal ScValid();
+    reveal ConnectionValid();
+    reveal NPsInSc();
+  }
+
+  lemma ConnectionKeysINPs(c: Circuit, e1: Entity, e2: Entity, connection: map<NP, NP>)
+    requires ScValid(c, e1.sc)
+    requires ScValid(c, e2.sc)
+    requires ConnectionValid(c, e1, e2, connection)
+    ensures INPsValid(c, connection.Keys)
+  {
+    reveal ScValid();
+    reveal ConnectionValid();
+    reveal NPsInSc();
+    reveal INPsValid();
+  }
+
+  lemma ConnectionValuesONPs(c: Circuit, e1: Entity, e2: Entity, connection: map<NP, NP>)
+    requires ScValid(c, e1.sc)
+    requires ScValid(c, e2.sc)
+    requires ConnectionValid(c, e1, e2, connection)
+    ensures ONPsValid(c, connection.Values)
+  {
+    reveal ScValid();
+    reveal ConnectionValid();
+    reveal NPsInSc();
+    reveal ONPsValid();
+  }
+
+  ghost predicate ConnectEntitiesRequirements(c: Circuit, e1: Entity, e2: Entity, connection: map<NP, NP>) {
+    && CircuitValid(c)
+    && EntityValid(c, e1)
+    && EntityValid(c, e2)
+    && IsIsland(c, e1.sc)
+    && IsIsland(c, e2.sc)
+    && SetsNoIntersection(e1.sc, e2.sc)
+    && ConnectionValid(c, e1, e2, connection)
+  }
+
+  lemma OtherNoIntersection(c: Circuit, e1: Entity, e2: Entity, connection: map<NP, NP>)
+    requires ConnectEntitiesRequirements(c, e1, e2, connection)
+    ensures SetsNoIntersection(AllInputs(c, e1.sc), AllInputs(c, e2.sc))
+    ensures SetsNoIntersection(AllPossibleOutputs(c, e1.sc), AllPossibleOutputs(c, e2.sc))
+  {
+    reveal NPsInSc();
+    reveal AllONPs();
+    reveal AllINPs();
+    reveal ConnInputs();
+    reveal ConnOutputs();
+    reveal UnconnInputs();
+    assert NPsInSc(e1.sc, AllInputs(c, e1.sc));
+    assert NPsInSc(e1.sc, AllPossibleOutputs(c, e1.sc));
+    assert NPsInSc(e2.sc, AllInputs(c, e2.sc));
+    assert NPsInSc(e2.sc, AllPossibleOutputs(c, e2.sc));
+    NPSetsNoIntersection(c, e1, e2, connection, AllInputs(c, e1.sc), AllInputs(c, e2.sc));
+    NPSetsNoIntersection(c, e1, e2, connection, AllPossibleOutputs(c, e1.sc), AllPossibleOutputs(c, e2.sc));
+  }
+
+  function ConnectEntitiesFInputs(c: Circuit, e1: Entity, e2: Entity, connection: map<NP, NP>): (r: set<NP>)
+    requires ConnectEntitiesRequirements(c, e1, e2, connection)
+    // The inputs into e1 and e2, minus any inputs into e1 that came from e1
+    ensures e1.finputs <= r
+  {
+    e1.finputs + (e2.finputs - connection.Keys)
+  }
+
+  function ConnectEntitiesF(c: Circuit, e1: Entity, e2: Entity, connection: map<NP, NP>,
+                            knowns: map<NP, bool>): (r: map<NP, bool>)
+    requires ConnectEntitiesRequirements(c, e1, e2, connection)
+    requires knowns.Keys == ConnectEntitiesFInputs(c, e1, e2, connection)
+    ensures r.Keys == e1.foutputs + e2.foutputs
+  {
+    var inputs_1 := ExtractMap(knowns, e1.finputs);
+    reveal EntityFValid();
+    assert inputs_1.Keys == e1.finputs;
+    assert e1.f.requires(inputs_1);
+    var outputs_1 := e1.f(inputs_1);
+    assert connection.Values <= outputs_1.Keys by { reveal ConnectionValid(); }
+    var outputs_1_to_2 := ExtractMap(outputs_1, connection.Values);
+    var inputs_2_from_1 := (map np | np in connection :: np := outputs_1_to_2[connection[np]]);
+    var combined_inputs := knowns + inputs_2_from_1;
+    var inputs_2 := ExtractMap(combined_inputs, e2.finputs);
+    var outputs_2 := e2.f(inputs_2);
+    assert outputs_2.Keys == e2.foutputs;
+    OtherNoIntersection(c, e1, e2, connection);
+    reveal EntitySomewhatValid();
+    FOutputsInSc(c, e1);
+    FOutputsInSc(c, e2);
+    NPSetsNoIntersection(c, e1, e2, connection, outputs_1.Keys, outputs_2.Keys);
+    var combined_outputs := AddMaps(outputs_1, outputs_2);
+    combined_outputs
+  }
+
+  lemma RearrangeKnownKeys(c: Circuit, e1: Entity, e2: Entity, connection: map<NP, NP>, knowns: map<NP, bool>)
+    requires ConnectEntitiesRequirements(c, e1, e2, connection)
+    requires knowns.Keys == e1.finputs + (e2.finputs - connection.Keys)
+    ensures knowns.Keys == (e1.finputs + e2.finputs) - connection.Keys
+  {
+    ConnectionKeysInE2(c, e1, e2, connection);
+    forall np | np in connection.Keys
+      ensures np !in e1.finputs
+    {
+      reveal NPsInSc();
+      assert np.n in e2.sc;
+      SetsNoIntersectionSymm(e1.sc, e2.sc);
+      InThisNotInThat(np.n, e2.sc, e1.sc);
+      assert np.n !in e1.sc;
+      FInputsInSc(c, e1);
+      assert np !in e1.finputs;
+    }
+  }
+
+  function CalculateE2Inputs(c: Circuit, e1: Entity, e2: Entity, connection: map<NP, NP>, knowns: map<NP, bool>): (r: map<NP, bool>)
+    requires ConnectEntitiesRequirements(c, e1, e2, connection)
+    requires knowns.Keys == e1.finputs + (e2.finputs - connection.Keys)
+  {
+    var inputs_1 := ExtractMap(knowns, e1.finputs);
+    reveal EntityFValid();
+    var outputs_1 := e1.f(inputs_1);
+    assert outputs_1.Keys == e1.foutputs;
+    reveal ConnectionValid();
+    assert connection.Values <= e1.foutputs;
+    var connected := (map np | np in connection :: np := outputs_1[connection[np]]);
+    assert connected.Keys == connection.Keys;
+    assert knowns.Keys == e1.finputs + (e2.finputs - connection.Keys);
+    RearrangeKnownKeys(c, e1, e2, connection, knowns);
+    assert knowns.Keys == (e1.finputs + e2.finputs) - connection.Keys;
+    var combined_map := AddMaps(knowns, connected);
+    var inputs_2 := ExtractMap(combined_map, e2.finputs);
+    inputs_2
+  }
+
+  lemma ConnectEntitiesFHelper(c: Circuit, e1: Entity, e2: Entity, connection: map<NP, NP>, knowns: map<NP, bool>, np: NP)
+    requires ConnectEntitiesRequirements(c, e1, e2, connection)
+    requires knowns.Keys == ConnectEntitiesFInputs(c, e1, e2, connection)
+    requires np in e2.foutputs
+    ensures
+      var knowns_2 := CalculateE2Inputs(c, e1, e2, connection, knowns);
+      && e2.f.requires(knowns_2)
+      && np in e2.f(knowns_2)
+      && e2.f(knowns_2)[np] == ConnectEntitiesF(c, e1, e2, connection, knowns)[np]
+  {
+    var inputs_1 := ExtractMap(knowns, e1.finputs);
+    reveal EntityFValid();
+    assert inputs_1.Keys == e1.finputs;
+    assert e1.f.requires(inputs_1);
+    var outputs_1 := e1.f(inputs_1);
+    assert connection.Values <= outputs_1.Keys by { reveal ConnectionValid(); }
+    var outputs_1_to_2 := ExtractMap(outputs_1, connection.Values);
+    var inputs_2_from_1 := (map np | np in connection :: np := outputs_1_to_2[connection[np]]);
+    var combined_inputs := knowns + inputs_2_from_1;
+    var inputs_2 := ExtractMap(combined_inputs, e2.finputs);
+
+    assert inputs_2 == CalculateE2Inputs(c, e1, e2, connection, knowns);
+
+    var outputs_2 := e2.f(inputs_2);
+    assert outputs_2.Keys == e2.foutputs;
+    OtherNoIntersection(c, e1, e2, connection);
+    reveal EntitySomewhatValid();
+    FOutputsInSc(c, e1);
+    FOutputsInSc(c, e2);
+    NPSetsNoIntersection(c, e1, e2, connection, outputs_1.Keys, outputs_2.Keys);
+    var combined_outputs := AddMaps(outputs_1, outputs_2);
+    assert combined_outputs == ConnectEntitiesF(c, e1, e2, connection, knowns);
+  }
+
+  opaque predicate ConnectCircuitRequirements(c: Circuit, connection: map<NP, NP>)
+  {
+    && (forall np :: np in connection.Keys ==> INPValid(c, np) && np !in c.PortSource)
+    && (forall np :: np in connection.Values ==> ONPValid(c, np))
+  }
+
+  function ConnectCircuit(c: Circuit, connection: map<NP, NP>): (r: Circuit)
+    requires CircuitValid(c)
+    requires ConnectCircuitRequirements(c, connection)
+    ensures CircuitValid(r)
+  {
+    reveal CircuitValid();
+    reveal ConnectCircuitRequirements();
+    var new_c := Circuit(
+      c.NodeKind,
+      AddMaps(c.PortSource, connection)
+    );
+    assert new_c.PortSource.Values == c.PortSource.Values + connection.Values;
+    assert (forall np :: np in new_c.PortSource.Values ==> ONPValid(new_c, np));
+    assert (forall np :: np in new_c.PortSource.Keys ==> INPValid(new_c, np));
+    new_c
+  }
+
+  lemma ConnectCircuitConservesSubcircuit(c: Circuit, connection: map<NP, NP>, sc: set<CNode>)
+    requires CircuitValid(c)
+    requires ConnectCircuitRequirements(c, connection)
+    requires ScValid(c, sc)
+    requires NoInternalConnections(connection, sc)
+    ensures SubcircuitConserved(c, ConnectCircuit(c, connection), sc)
+  {
+    reveal NoInternalConnections();
+    var ca := c;
+    var cb := ConnectCircuit(c, connection);
+    reveal ScValid();
+    assert (forall n :: n in sc ==> n in cb.NodeKind);
+    assert (forall n :: n in sc ==> ca.NodeKind[n] == cb.NodeKind[n]);
+    assert (forall np: NP :: np.n in sc && np in ca.PortSource ==>
+            np in cb.PortSource && ca.PortSource[np] == cb.PortSource[np]);
+    assert (forall np: NP :: np.n in sc && np !in ca.PortSource && np in cb.PortSource ==>
+        cb.PortSource[np].n !in sc);
+    reveal SubcircuitConserved();
+  }
+
+  opaque predicate NoInternalConnections(connection: map<NP, NP>, sc: set<CNode>)
+  {
+    && (forall np :: np in connection.Keys && np.n in sc ==> connection[np].n !in sc)
+  }
+
+  opaque predicate ConnectionValuesInFOutputs(connection: map<NP, NP>, e: Entity)
+  {
+    && (forall np :: np in connection.Values && np.n in e.sc ==> np in e.foutputs)
+  }
+
+  predicate ConnectionsEntityCompatible(connection: map<NP, NP>, e: Entity)
+  {
+    && NoInternalConnections(connection, e.sc)
+    && ConnectionValuesInFOutputs(connection, e)
+  }
+
+
+
+  lemma ConnectCircuitEntitiesStillValid(c: Circuit, connection: map<NP, NP>, e: Entity)
+    requires CircuitValid(c)
+    requires ConnectCircuitRequirements(c, connection)
+    requires EntityValid(c, e)
+    requires ConnectionsEntityCompatible(connection, e)
+    ensures EntityValid(ConnectCircuit(c, connection), e)
+  {
+    reveal NoInternalConnections();
+    var new_c := ConnectCircuit(c, connection);
+    ConnectCircuitConservesSubcircuit(c, connection, e.sc);
+    assert ScValid(new_c, e.sc) by {
+      reveal ScValid();
+    }
+    assert OutputsInFOutputs(new_c, e) by {
+      reveal ConnOutputs();
+      reveal EntitySomewhatValid();
+      assert OutputsInFOutputs(c, e);
+      reveal ConnectionValuesInFOutputs();
+    }
+    EntityConserved(c, new_c, e);
+  }
+
+  lemma ConnectEntitiesIsIsland(c: Circuit, e1: Entity, e2: Entity, connection: map<NP, NP>)
+    requires ConnectEntitiesRequirements(c, e1, e2, connection)
+    ensures
+      var (new_c, e) := ConnectEntitiesImpl(c, e1, e2, connection);
+      IsIsland(new_c, e.sc)
+  {
+    reveal NPsInSc();
+    var (new_c, e) := ConnectEntitiesImpl(c, e1, e2, connection);
+    var sc1 := e1.sc;
+    var sc2 := e2.sc;
+    assert ScValid(c, sc1 + sc2) by {
+      reveal ScValid();
+    }
+    var sco := SubcircuitComplement(c, sc1 + sc2);
+    assert |sco * sc1| == 0;
+    assert |sco * sc2| == 0;
+
+    assert IsIsland(c, sc1);
+    assert IsIsland(c, sc2);
+    assert IsIsland(c, sc1 + sc2) by {
+      reveal IsIsland();
+    }
+    assert IsIsland(c, sco) by {
+      reveal ScValid();
+      IsIslandComplementIsIsland(c, sc1+sc2);
+    }
+
+    assert NoConnFromTo(c, sc1, sc2) by {reveal ScValid(); IsIslandNoConns(c, sc1, sc2);}
+    assert NoConnFromTo(c, sc1, sco) by {reveal ScValid(); IsIslandNoConns(c, sc1, sco);}
+    assert NoConnFromTo(c, sc2, sc1) by {reveal ScValid(); IsIslandNoConns(c, sc2, sc1);}
+    assert NoConnFromTo(c, sc2, sco) by {reveal ScValid(); IsIslandNoConns(c, sc2, sco);}
+    assert NoConnFromTo(c, sco, sc1) by {reveal ScValid(); IsIslandNoConns(c, sco, sc1);}
+    assert NoConnFromTo(c, sco, sc2) by {reveal ScValid(); IsIslandNoConns(c, sco, sc2);}
+
+    forall np: NP | np in new_c.PortSource
+      ensures np.n in sc1+sc2 ==> new_c.PortSource[np].n in sc1+sc2
+      ensures np.n !in sc1+sc2 ==> new_c.PortSource[np].n !in sc1+sc2
+    {
+      reveal CircuitValid();
+      reveal ConnectionValid();
+      reveal IsIsland();
+      reveal ConnectEntitiesImpl();
+      assert NodeValid(c, np.n);
+      InScOrComplement(c, sc1+sc2, np.n);
+      if np !in connection {
+        assert new_c.PortSource[np] == c.PortSource[np];
+      }
+      if np.n in sc1 {
+        assert np !in connection.Keys;
+        assert new_c.PortSource[np] == c.PortSource[np];
+        assert new_c.PortSource[np].n in sc1;
+      } else if np.n in sc2 {
+        assert np !in connection.Values;
+        if np in connection.Keys {
+          assert new_c.PortSource[np] == connection[np];
+          ConnectionValuesInE1(c, e1, e2, connection);
+          assert connection[np].n in sc1;
+          assert new_c.PortSource[np].n in sc1;
+        } else {
+          assert new_c.PortSource[np] == c.PortSource[np];
+        }
+        assert new_c.PortSource[np].n in sc1 + sc2;
+      } else {
+        assert np.n in sco;
+        assert np !in connection.Keys;
+        assert np !in connection.Values;
+        assert new_c.PortSource[np] == c.PortSource[np];
+        assert new_c.PortSource[np].n !in sc1;
+        assert new_c.PortSource[np].n !in sc2;
+      }
+    }
+    reveal IsIsland();
+    assert e.sc == sc1 + sc2 by {
+      reveal ConnectEntitiesImpl();
+    }
+    assert (forall np :: np in new_c.PortSource && np.n in e.sc ==> new_c.PortSource[np].n in e.sc);
+    assert (forall np :: np in new_c.PortSource && np.n !in e.sc ==> new_c.PortSource[np].n !in e.sc);
+    assert IsIsland(new_c, e.sc);
+  }
+
+  lemma ConnectCircuitReqFromConnectEntitiesReq(c: Circuit, e1: Entity, e2: Entity, connection: map<NP, NP>)
+    requires ConnectEntitiesRequirements(c, e1, e2, connection)
+    ensures ConnectCircuitRequirements(c, connection)
+  {
+    reveal ConnectionValid();
+    reveal EntitySomewhatValid();
+    reveal ConnectCircuitRequirements();
+    ConnectionKeysINPs(c, e1, e2, connection);
+    ConnectionValuesONPs(c, e1, e2, connection);
+    reveal INPsValid();
+    reveal ONPsValid();
+    SetsNoIntersectionDuh(connection.Keys, c.PortSource.Keys);
+    assert (forall np :: np in connection.Keys ==> INPValid(c, np) && np !in c.PortSource);
+    assert (forall np :: np in connection.Values ==> ONPValid(c, np));
+  }
+
+  opaque function ConnectEntitiesImpl(
+      c: Circuit, e1: Entity, e2: Entity, connection: map<NP, NP>): (r: (Circuit, Entity))
+    requires ConnectEntitiesRequirements(c, e1, e2, connection)
+    ensures CircuitValid(r.0)
+  {
+    var new_finputs := ConnectEntitiesFInputs(c, e1, e2, connection);
+    var new_f := (knowns: map<NP, bool>) requires knowns.Keys == new_finputs =>
+      ConnectEntitiesF(c, e1, e2, connection, knowns);
+    var e := Entity(
+      e1.sc + e2.sc,
+      new_finputs,
+      e1.foutputs + e2.foutputs,
+      new_f
+    );
+
+    assert ConnectCircuitRequirements(c, connection) by {
+      ConnectCircuitReqFromConnectEntitiesReq(c, e1, e2, connection);
+    }
+    var new_c := ConnectCircuit(c, connection);
+    (new_c, e)
+  }
+
+  lemma ConnectEntitiesScValid(c: Circuit, e1: Entity, e2: Entity, connection: map<NP, NP>)
+    requires ConnectEntitiesRequirements(c, e1, e2, connection)
+    ensures
+      var (new_c, e) := ConnectEntitiesImpl(c, e1, e2, connection);
+      ScValid(new_c, e.sc)
+  {
+    reveal ConnectEntitiesImpl();
+    reveal ScValid();
+  }
+
+  lemma ConnectEntitiesFOutputsCorrect(c: Circuit, e1: Entity, e2: Entity, connection: map<NP, NP>)
+    requires ConnectEntitiesRequirements(c, e1, e2, connection)
+    ensures
+      var (new_c, e) := ConnectEntitiesImpl(c, e1, e2, connection);
+      && ScValid(new_c, e.sc)
+      && (AllPossibleOutputs(new_c, e.sc) >= e.foutputs >= AllOutputs(new_c, e.sc))
+  {
+    var (new_c, e) := ConnectEntitiesImpl(c, e1, e2, connection);
+    reveal ScValid();
+    reveal ConnectEntitiesImpl();
+    reveal AllONPs();
+    reveal SeqOutputs();
+    reveal FinalOutputs();
+    assert AllOutputs(c, e.sc) == AllOutputs(c, e1.sc) + AllOutputs(c, e2.sc) by {
+      reveal IsIsland();
+      reveal ConnOutputs();
+    }
+    assert AllPossibleOutputs(new_c, e.sc) == AllPossibleOutputs(c, e1.sc) + AllPossibleOutputs(c, e2.sc);
+    assert ConnOutputs(c, e1.sc) == {} by {
+      reveal IsIsland();
+      reveal ConnOutputs();
+    }
+    ConnectEntitiesIsIsland(c, e1, e2,  connection);
+    IsIslandNoOutputs(new_c, e.sc);
+    IsIslandNoOutputs(c, e1.sc);
+    IsIslandNoOutputs(c, e2.sc);
+
+    assert e.foutputs >= AllOutputs(c, e1.sc) + AllOutputs(c, e2.sc) by {reveal EntitySomewhatValid();}
+    assert e.foutputs <= AllPossibleOutputs(c, e1.sc) + AllPossibleOutputs(c, e2.sc) by {reveal EntitySomewhatValid();}
+
+    assert AllPossibleOutputs(c, e.sc) >= e.foutputs >= AllOutputs(c, e.sc) by {reveal EntitySomewhatValid();}
+  }
+
+  lemma NPSetsNoIntersection(c: Circuit, e1: Entity, e2: Entity, connection: map<NP, NP>, nps1: set<NP>, nps2: set<NP>)
+    requires ConnectEntitiesRequirements(c, e1, e2, connection)
+    requires NPsInSc(e1.sc, nps1)
+    requires NPsInSc(e2.sc, nps2)
+    ensures SetsNoIntersection(nps1, nps2)
+  {
+    reveal NPsInSc();
+    if exists np :: np in nps1 && np in nps2 {
+      var np :| np in nps1 && np in nps2;
+      assert np.n in e1.sc && np.n in e2.sc;
+      assert SetsNoIntersection(e1.sc, e2.sc);
+      NotInBoth(np.n, e1.sc, e2.sc);
+      assert false;
+    }
+  }
+
+  lemma ReorderSets<T>(a: set<T>, b: set<T>, c: set<T>)
+    requires SetsNoIntersection(b, c)
+    ensures (a - b) + c == (a + c) - b
+  {
+    SetsNoIntersectionDuh(b, c);
+    assert !exists x :: x in b && x in c;
+  }
+
+  lemma ReorderSets2<T>(a: set<T>, b: set<T>, c: set<T>)
+    requires SetsNoIntersection(a, c)
+    ensures (a + b) - c == a + (b - c)
+  {
+    SetsNoIntersectionDuh(a, c);
+    assert !exists x :: x in a && x in c;
+  }
+
+  lemma ConnectEntitiesSomewhatValid(c: Circuit, e1: Entity, e2: Entity, connection: map<NP, NP>)
+    requires ConnectEntitiesRequirements(c, e1, e2, connection)
+    ensures
+      var (new_c, e) := ConnectEntitiesImpl(c, e1, e2, connection);
+      EntitySomewhatValid(new_c, e)
+  {
+    var (new_c, e) := ConnectEntitiesImpl(c, e1, e2, connection);
+    ConnectEntitiesFOutputsCorrect(c, e1, e2, connection);
+
+    calc {
+      AllInputs(new_c, e.sc) == UnconnInputs(new_c, e.sc) + ConnInputs(new_c, e.sc) + SeqInputs(new_c, e.sc) + FinalInputs(new_c, e.sc);
+      {
+        reveal ScValid();
+        reveal UnconnInputs();
+        reveal ConnectEntitiesImpl();
+        assert UnconnInputs(new_c, e.sc) == UnconnInputs(c, e.sc)-connection.Keys;
+      }
+      AllInputs(new_c, e.sc) == (UnconnInputs(c, e.sc)-connection.Keys) + ConnInputs(new_c, e.sc) + SeqInputs(new_c, e.sc) + FinalInputs(new_c, e.sc);
+      {
+        ConnectEntitiesIsIsland(c, e1, e2,  connection);
+        IsIslandNoInputs(new_c, e.sc);
+        reveal IsIsland();
+        reveal ConnInputs();
+        assert |ConnInputs(new_c, e.sc)| == 0;
+      }
+      AllInputs(new_c, e.sc) == (UnconnInputs(c, e.sc)-connection.Keys) + SeqInputs(new_c, e.sc) + FinalInputs(new_c, e.sc);
+      {
+        reveal SeqInputs();
+        reveal FinalInputs();
+        reveal ConnectEntitiesImpl();
+        assert SeqInputs(new_c, e.sc) == SeqInputs(c, e.sc);
+        assert FinalInputs(new_c, e.sc) == FinalInputs(c, e.sc);
+      }
+      AllInputs(new_c, e.sc) == (UnconnInputs(c, e.sc)-connection.Keys) + SeqInputs(c, e.sc) + FinalInputs(c, e.sc);
+      {
+        UnconnInputsAdd(c, e1.sc, e2.sc);
+        reveal ConnectEntitiesImpl();
+        assert UnconnInputs(c, e.sc) == UnconnInputs(c, e1.sc) + UnconnInputs(c, e2.sc);
+        reveal SeqInputs();
+        reveal FinalInputs();
+        assert SeqInputs(c, e.sc) == SeqInputs(c, e1.sc) + SeqInputs(c, e2.sc);
+        assert FinalInputs(c, e.sc) == FinalInputs(c, e1.sc) + FinalInputs(c, e2.sc);
+      }
+      AllInputs(new_c, e.sc) == ((UnconnInputs(c, e1.sc)+UnconnInputs(c, e2.sc))-connection.Keys) +
+                                 SeqInputs(c, e1.sc) + SeqInputs(c, e2.sc) + FinalInputs(c, e1.sc) + FinalInputs(c, e2.sc);
+      {
+        ConnectionKeysInE2(c, e1, e2, connection);
+        NPSetsNoIntersection(c, e1, e2, connection, UnconnInputs(c, e1.sc), connection.Keys);
+        assert |UnconnInputs(c, e1.sc) * connection.Keys| == 0;
+        ReorderSets2(UnconnInputs(c, e1.sc), UnconnInputs(c, e2.sc), connection.Keys);
+      }
+      AllInputs(new_c, e.sc) == UnconnInputs(c, e1.sc)+(UnconnInputs(c, e2.sc)-connection.Keys) +
+                                 SeqInputs(c, e1.sc) + SeqInputs(c, e2.sc) + FinalInputs(c, e1.sc) + FinalInputs(c, e2.sc);
+      AllInputs(new_c, e.sc) == (UnconnInputs(c, e1.sc) + SeqInputs(c, e1.sc) + FinalInputs(c, e1.sc)) +
+                                ((UnconnInputs(c, e2.sc)-connection.Keys) + SeqInputs(c, e2.sc) + FinalInputs(c, e2.sc));
+      {
+        ConnectionKeysINPs(c, e1, e2, connection);
+        INPsAndONPsNoIntersection(c, connection.Keys, SeqInputs(c, e2.sc));
+        INPsAndONPsNoIntersection(c, connection.Keys, FinalInputs(c, e2.sc));
+        SetsNoIntersectionAdds(connection.Keys, SeqInputs(c, e2.sc), FinalInputs(c, e2.sc));
+        ReorderSets(UnconnInputs(c, e2.sc), connection.Keys, SeqInputs(c, e2.sc) + FinalInputs(c, e2.sc));
+        assert ((UnconnInputs(c, e2.sc)-connection.Keys) + SeqInputs(c, e2.sc) + FinalInputs(c, e2.sc)) ==
+               ((UnconnInputs(c, e2.sc) + SeqInputs(c, e2.sc) + FinalInputs(c, e2.sc)) - connection.Keys);
+      }
+      AllInputs(new_c, e.sc) == (UnconnInputs(c, e1.sc) + SeqInputs(c, e1.sc) + FinalInputs(c, e1.sc)) +
+                                ((UnconnInputs(c, e2.sc) + SeqInputs(c, e2.sc) + FinalInputs(c, e2.sc)) - connection.Keys);
+      {
+        reveal IsIsland();
+        reveal ConnInputs();
+        assert |ConnInputs(c, e1.sc)| == 0;
+        assert |ConnInputs(c, e2.sc)| == 0;
+        assert AllInputs(c, e1.sc) == (UnconnInputs(c, e1.sc) + SeqInputs(c, e1.sc) + FinalInputs(c, e1.sc));
+        assert AllInputs(c, e2.sc) == (UnconnInputs(c, e2.sc) + SeqInputs(c, e2.sc) + FinalInputs(c, e2.sc));
+      }
+      AllInputs(new_c, e.sc) == AllInputs(c, e1.sc) + (AllInputs(c, e2.sc) - connection.Keys);
+      {
+        reveal EntitySomewhatValid();
+      }
+      AllInputs(new_c, e.sc) == e1.finputs + (e2.finputs - connection.Keys);
+      {
+        reveal ConnectEntitiesImpl();
+      }
+      AllInputs(new_c, e.sc) == e.finputs;
+    }
+    reveal EntitySomewhatValid();
+    assert EntitySomewhatValid(new_c, e);
+  }
+
+  lemma ConnectEntitiesFValid(c: Circuit, e1: Entity, e2: Entity, connection: map<NP, NP>)
+    requires ConnectEntitiesRequirements(c, e1, e2, connection)
+    ensures
+      var (new_c, e) := ConnectEntitiesImpl(c, e1, e2, connection);
+      EntityFValid(new_c, e)
+  {
+    reveal ConnectEntitiesImpl();
+    reveal EntityFValid();
+  }
+
+  lemma ConnectEntitiesEntitiesStillValid(c: Circuit, e1: Entity, e2: Entity, connection: map<NP, NP>)
+    requires ConnectEntitiesRequirements(c, e1, e2, connection)
+    ensures
+      && ConnectCircuitRequirements(c, connection)
+      && var new_c := ConnectEntitiesImpl(c, e1, e2, connection).0;
+      && EntityValid(new_c, e1)
+      && EntityValid(new_c, e2)
+  {
+    var new_c := ConnectEntitiesImpl(c, e1, e2, connection).0;
+    ConnectCircuitReqFromConnectEntitiesReq(c, e1, e2, connection);
+    assert new_c == ConnectCircuit(c, connection) by {
+      reveal ConnectEntitiesImpl();
+    }
+    ConnectCircuitReqFromConnectEntitiesReq(c, e1, e2, connection);
+    assert NoInternalConnections(connection, e1.sc) by {
+      reveal NoInternalConnections();
+      reveal ConnectionValid();
+      assert (connection.Keys <= e2.finputs * AllINPs(c, e2.sc));
+      assert (connection.Values <= e1.foutputs * AllONPs(c, e1.sc));
+      ConnectionKeysInE2(c, e1, e2, connection);
+      forall np | np in connection.Keys
+        ensures np.n !in e1.sc
+      {
+        assert SetsNoIntersection(e1.sc, e2.sc);
+        SetsNoIntersectionSymm(e1.sc, e2.sc);
+        reveal NPsInSc();
+        assert np.n in e2.sc;
+        InThisNotInThat(np.n, e2.sc, e1.sc);
+      }
+    }
+    assert ConnectionValuesInFOutputs(connection, e1) by {
+      reveal ConnectionValuesInFOutputs();
+      reveal ConnectionValid();
+    }
+    ConnectCircuitEntitiesStillValid(c, connection, e1);
+    assert ConnectionsEntityCompatible(connection, e1);
+    assert NoInternalConnections(connection, e2.sc) by {
+      reveal NoInternalConnections();
+      reveal ConnectionValid();
+      assert (connection.Keys <= e2.finputs * AllINPs(c, e2.sc));
+      assert (connection.Values <= e1.foutputs * AllONPs(c, e1.sc));
+      ConnectionValuesInE1(c, e1, e2, connection);
+      forall np | np in connection.Values
+        ensures np.n !in e2.sc
+      {
+        assert SetsNoIntersection(e1.sc, e2.sc);
+        reveal NPsInSc();
+        assert np.n in e1.sc;
+        InThisNotInThat(np.n, e1.sc, e2.sc);
+      }
+    }
+    assert ConnectionValuesInFOutputs(connection, e2) by {
+      ConnectionValuesInE1(c, e1, e2, connection);
+      forall np | np in connection.Values
+        ensures np.n !in e2.sc
+      {
+        reveal NPsInSc();
+        assert np.n in e1.sc;
+        InThisNotInThat(np.n, e1.sc, e2.sc);
+      }
+      reveal ConnectionValuesInFOutputs();
+    }
+    assert ConnectionsEntityCompatible(connection, e2);
+    ConnectCircuitEntitiesStillValid(c, connection, e2);
+  }
+
+  //lemma ConnectEntitiesValid(c: Circuit, e1: Entity, e2: Entity, connection: map<NP, NP>)
+  //  requires ConnectEntitiesRequirements(c, e1, e2, connection)
+  //  ensures
+  //    var (new_c, e) := ConnectEntitiesImpl(c, e1, e2, connection);
+  //    EntityEvaluatesCorrectly(new_c, e)
+  //{
+  //  //reveal ConnectEntitiesImpl();
+  //  var (new_c, e) := ConnectEntitiesImpl(c, e1, e2, connection);
+  //  forall knowns: map<NP, bool> | knowns.Keys == e.finputs {
+  //    forall np | np in e.foutputs {
+  //      assert Evaluate(c, np, knowns) == EvalOk(e.f(knowns)[np]);
+  //    }
+  //  }
+  //}
+
+  //lemma SetsNoIntersectionFromComposedValid(c: Circuit, e1: Entity, e2: Entity)
+  //requires ComposedValid(c, e1, e2)
+  //ensures SetsNoIntersection(e1.sc, e2.sc)
+  //ensures SetsNoIntersection(e1.finputs, e2.finputs)
+  //ensures SetsNoIntersection(e1.foutputs, e2.foutputs)
+  //ensures SetsNoIntersection(e1.finputs, e2.foutputs)
+  //ensures SetsNoIntersection(e1.foutputs, e2.finputs)
+  //{
+  //  reveal ScValid();
+  //  
+  //  //reveal EntityValid();
+  //  //reveal NPsValidAndInSc();
+  //}
+
+  //function ComposeEntity(c: Circuit, e1: Entity, e2: Entity): (r: Entity)
+  //  requires ComposedValid(c, e1, e2)
+  //  ensures EntityValid(c, r)
+  //{
+  //  var combined_input_keys := ComposeEntityInputs(c, e1, e2);
+  //  var e := Entity(
+  //    CombineSets(e1.sc, e2.sc),
+  //    combined_input_keys,
+  //    e1.foutputs + e2.foutputs,
+  //    (combined_inputs: map<NP, bool>) requires combined_inputs.Keys == combined_input_keys =>
+  //      ComposeEntityF(c, e1, e2, combined_inputs)
+  //  );
+  //  assert ScValid(c, e.sc) by {reveal ScValid();}
+  //  assert (ScInputBoundary(c, e.sc) == e.finputs) by {
+  //    ComposeEntityInputsCorrect(c, e1, e2);
+  //  }
+  //  assert SetsNoIntersection(e.finputs, e.foutputs) by {
+  //    SetsNoIntersectionFromComposedValid(c, e1, e2);
+  //  }
+  //  //assert NPsValidAndInSc(c, e.sc, e.outputs) by {reveal NPsValidAndInSc();}
+  //  //assert NPsValidAndInSc(c, e.sc, e.inputs) by {reveal NPsValidAndInSc();}
+  //  //assert MapFunctionValid(EtoMf(e)) by {reveal MapFunctionValid();}
+  //  //assert EntityScOutputsInOutputs(c, e.sc, e.outputs) by {reveal EntityScOutputsInOutputs();}
+  //  //assert EntityValid(c, e);
+  //  e
+  //}
+
+  //function ComposeEntityInputs(c: Circuit, e1: Entity, e2: Entity): (r: set<NP>)
+  //  requires ComposedValid(c, e1, e2)
+  //  ensures forall np :: np in e1.finputs ==> np in r
+  //{
+  //  (e1.finputs + e2.finputs) - NPBetweenSubcircuits(c, e2.sc, e1.sc)
+  //}
+
+  //lemma {:vcs_split_on_every_assert} ComposeEntityInputsCorrectHelper(c: Circuit, e1: Entity, e2: Entity)
+  //  requires ComposedValid(c, e1, e2)
+  //  ensures
+  //    ScValid(c, e1.sc) &&
+  //    ScValid(c, e2.sc) &&
+  //    ScValid(c, e1.sc + e2.sc) &&
+  //    NPBetweenSubcircuitsComplement(c, e1.sc + e2.sc, e1.sc + e2.sc) ==
+  //      NPBetweenSubcircuitsComplement(c, e1.sc, e1.sc) +
+  //      NPBetweenSubcircuitsComplement(c, e2.sc, e2.sc) -
+  //      NPBetweenSubcircuits(c, e2.sc, e1.sc)
+  //{
+  //  assert ScValid(c, e1.sc);
+  //  assert ScValid(c, e2.sc);
+  //  assert ScValid(c, e1.sc + e2.sc) by {reveal ScValid();}
+  //  assert NPBetweenSubcircuitsComplement(c, e1.sc + e2.sc, e1.sc + e2.sc) ==
+  //      NPBetweenSubcircuitsComplement(c, e1.sc, e1.sc) + NPBetweenSubcircuitsComplement(c, e2.sc, e2.sc) -
+  //      NPBetweenSubcircuits(c, e2.sc, e1.sc) - NPBetweenSubcircuits(c, e1.sc, e2.sc);
+  //  assert NPBetweenSubcircuits(c, e1.sc, e2.sc) == {};
+  //}
+
+  //lemma ComposeEntityInputsCorrect(c: Circuit, e1: Entity, e2: Entity)
+  //  requires ComposedValid(c, e1, e2)
+  //  ensures ScValid(c, e1.sc + e2.sc)
+  //  ensures
+  //    ScInputBoundary(c, e1.sc + e2.sc) == ComposeEntityInputs(c, e1, e2)
+  //{
+  //  assert ScValid(c, e1.sc + e2.sc) && ScValid(c, e1.sc) && ScValid(c, e2.sc) by {
+  //    reveal ScValid();
+  //  }
+  //  var ui := UnconnectedINPs(c, e1.sc + e2.sc) + InternalInputs(c, e1.sc + e2.sc);
+  //  var nb :=  NPBetweenSubcircuitsComplement(c, e1.sc, e1.sc) +
+  //             NPBetweenSubcircuitsComplement(c, e2.sc, e2.sc) -
+  //             NPBetweenSubcircuits(c, e2.sc, e1.sc);
+  //  calc {
+  //    ComposeEntityInputs(c, e1, e2);
+  //    (e1.finputs + e2.finputs) - NPBetweenSubcircuits(c, e2.sc, e1.sc);
+  //    //{reveal EntityValid();}
+  //    ScInputBoundary(c, e1.sc) + ScInputBoundary(c, e2.sc)
+  //      - NPBetweenSubcircuits(c, e2.sc, e1.sc);
+  //    NPBetweenSubcircuitsComplement(c, e1.sc, e1.sc) +
+  //      UnconnectedINPs(c, e1.sc) + InternalInputs(c, e1.sc) +
+  //      NPBetweenSubcircuitsComplement(c, e2.sc, e2.sc) +
+  //      UnconnectedINPs(c, e2.sc) + InternalInputs(c, e2.sc) -
+  //      NPBetweenSubcircuits(c, e2.sc, e1.sc);
+  //    UnconnectedINPs(c, e1.sc + e2.sc) + InternalInputs(c, e1.sc + e2.sc) +
+  //      NPBetweenSubcircuitsComplement(c, e1.sc, e1.sc) +
+  //      NPBetweenSubcircuitsComplement(c, e2.sc, e2.sc) -
+  //      NPBetweenSubcircuits(c, e2.sc, e1.sc);
+  //    {
+  //      // Need to show that the terms in NPBetweenSubcircuits are not in Unconnected or Internal.
+  //      assert forall np :: np in UnconnectedINPs(c, e1.sc + e2.sc) ==> np !in c.PortSource;
+  //      reveal CircuitValid();
+  //      assert forall np :: np in InternalInputs(c, e1.sc + e2.sc) ==> np !in c.PortSource;
+  //      assert forall np :: np in NPBetweenSubcircuits(c, e2.sc, e1.sc) ==> np in c.PortSource;
+  //    }
+  //    UnconnectedINPs(c, e1.sc + e2.sc) + InternalInputs(c, e1.sc + e2.sc) +
+  //      (NPBetweenSubcircuitsComplement(c, e1.sc, e1.sc) +
+  //      NPBetweenSubcircuitsComplement(c, e2.sc, e2.sc) -
+  //      NPBetweenSubcircuits(c, e2.sc, e1.sc));
+  //    {ComposeEntityInputsCorrectHelper(c, e1, e2);}
+  //    UnconnectedINPs(c, e1.sc + e2.sc) + InternalInputs(c, e1.sc + e2.sc) +
+  //      NPBetweenSubcircuitsComplement(c, e1.sc + e2.sc, e1.sc + e2.sc);
+  //    ScInputBoundary(c, e1.sc + e2.sc);
+  //  }
+  //}
+
+  //lemma ONPNotInKnownsNotInKnowns2(c: Circuit, onp: NP, e1: Entity, e2: Entity, knowns: map<NP, bool>)
+  //  requires ComposedValid(c, e1, e2)
+  //  requires GoodKnownKeys(c, e1, e2, knowns)
+  //  requires onp !in knowns
+  //  requires ONPValid(c, onp)
+  //  ensures onp !in CalculateE2Inputs(c, e1, e2, knowns)
+  //{
+  //  reveal GoodKnownKeys();
+  //  assert (onp !in (e1.finputs + e2.finputs) - NPBetweenSubcircuits(c, e2.sc, e1.sc));
+  //  var knowns_2 := CalculateE2Inputs(c, e1, e2, knowns);
+  //  var e2_inputs_from_e1_keys := NPBetweenSubcircuits(c, e2.sc, e1.sc);
+  //  assert forall np :: np in knowns_2 ==> np in e2_inputs_from_e1_keys || np in knowns;
+  //  assert onp !in e2_inputs_from_e1_keys by {
+  //    reveal CircuitValid();
+  //  }
+  //}
+
+  //opaque predicate GoodKnownKeys(c: Circuit, e1: Entity, e2: Entity, knowns: map<NP, bool>)
+  //  requires ComposedValid(c, e1, e2)
+  //{
+  //  knowns.Keys == ComposeEntityInputs(c, e1, e2)
+  //}
+
+  //lemma InE1ButNotE1InputsNotInKnowns(c: Circuit, e1: Entity, e2: Entity, knowns: map<NP, bool>, np: NP)
+  //  requires ComposedValid(c, e1, e2)
+  //  requires GoodKnownKeys(c, e1, e2, knowns)
+  //  requires np.n in e1.sc
+  //  requires np !in e1.finputs
+  //  ensures np !in knowns
+  //{
+  //  reveal GoodKnownKeys();
+  //  reveal ScValid();
+  //  InThisNotInThat(np.n, e1.sc, e2.sc);
+  //  assert np.n !in e2.sc;
+  //  assert knowns.Keys == (e1.finputs + e2.finputs) - NPBetweenSubcircuits(c, e2.sc, e1.sc);
+  //  //reveal EntityValid();
+  //  //reveal NPsValidAndInSc();
+  //  assert np !in e2.finputs;
+  //}
+
+  //lemma InE2ButNotE2InputsNotInKnowns(c: Circuit, e1: Entity, e2: Entity, knowns: map<NP, bool>, np: NP)
+  //  requires ComposedValid(c, e1, e2)
+  //  requires GoodKnownKeys(c, e1, e2, knowns)
+  //  requires np.n in e2.sc
+  //  requires np !in e2.finputs
+  //  ensures np !in knowns
+  //{
+  //  reveal GoodKnownKeys();
+  //  reveal ScValid();
+  //  InThisNotInThat(np.n, e2.sc, e1.sc);
+  //  assert np.n !in e1.sc;
+  //  assert knowns.Keys == (e1.finputs + e2.finputs) - NPBetweenSubcircuits(c, e2.sc, e1.sc);
+  //  //reveal EntityValid();
+  //  //reveal NPsValidAndInSc();
+  //  assert np !in e2.finputs;
+  //}
+
+  //function CalculateE2Inputs(c: Circuit, e1: Entity, e2: Entity, knowns: map<NP, bool>): (r: map<NP, bool>)
+  //  requires ComposedValid(c, e1, e2)
+  //  requires GoodKnownKeys(c, e1, e2, knowns)
+  //{
+  //  reveal CircuitValid();
+  //  reveal GoodKnownKeys();
+  //  //var mf1 := EtoMf(e1);
+  //  //var mf2 := EtoMf(e2);
+  //  //assert MapFunctionValid(mf1);
+  //  //assert MapFunctionValid(mf2);
+  //  var e2_inputs_from_e1_keys := NPBetweenSubcircuits(c, e2.sc, e1.sc);
+  //  var e2_inputs_from_e1 := (map np | np in e2_inputs_from_e1_keys :: np := c.PortSource[np]);
+  //  assert forall np :: np in e2_inputs_from_e1_keys ==> np in e2.finputs;
+  //  //assert forall np :: np in e2_inputs_from_e1.Values ==> np in e1.foutputs by {
+  //  //  reveal EntityScOutputsInOutputs();
+  //  //}
+  //  ////assert SetsNoIntersection(mf1.inputs+mf1.outputs, mf2.inputs+mf2.outputs) by {
+  //  ////  reveal NPsValidAndInSc();
+  //  ////}
+  //  //GetInputs2(mf1, mf2, e2_inputs_from_e1, knowns)
+  //  map[]
+  //}
+
+  //lemma CalculateE2InputsKeysCorrect(c: Circuit, e1: Entity, e2: Entity, knowns: map<NP, bool>)
+  //  requires ComposedValid(c, e1, e2)
+  //  requires GoodKnownKeys(c, e1, e2, knowns)
+  //  ensures
+  //    CalculateE2Inputs(c, e1, e2, knowns).Keys == e2.finputs
+  //{
+  //}
+
+  //function ComposeEntityF(c: Circuit, e1: Entity, e2: Entity, combined_inputs: map<NP, bool>): (r: map<NP, bool>)
+  //  requires ComposedValid(c, e1, e2)
+  //  requires combined_inputs.Keys == ComposeEntityInputs(c, e1, e2)
+  //{
+  //  //reveal EntityValid();
+  //  //var mf1 := MapFunction(e1.finputs, e1.foutputs, e1.f);
+  //  //var mf2 := MapFunction(e2.finputs, e2.foutputs, e2.f);
+  //  //assert MapFunctionValid(mf1);
+  //  //assert MapFunctionValid(mf2);
+  //  var e2_inputs_from_e1_keys := NPBetweenSubcircuits(c, e2.sc, e1.sc);
+  //  var e2_inputs_from_e1 := (map np | np in e2_inputs_from_e1_keys :: np := c.PortSource[np]);
+  //  assert forall np :: np in e2_inputs_from_e1_keys ==> np in e2.finputs by {
+  //    reveal CircuitValid();
+  //  }
+  //  assert forall np :: np in e2_inputs_from_e1.Values ==> np in e1.foutputs by {
+  //    //reveal EntityScOutputsInOutputs();
+  //    reveal CircuitValid();
+  //  }
+  //  //assert SetsNoIntersection(mf1.inputs+mf1.outputs, mf2.inputs+mf2.outputs) by {
+  //  //  //reveal NPsValidAndInSc();
+  //  //}
+  //  //ComposeMapFunction(mf1, mf2, e2_inputs_from_e1, combined_inputs)
+  //  map[]
+  //}
+}
