Attempt2/Entity.dfy
@@ -1,0 +1,158 @@
+module Entity {
+
+  import opened Subcircuit
+  import opened Circ
+  import opened Eval
+  import opened Utils
+  import opened MapFunction
+
+  datatype Entity = Entity(
+    sc: set<CNode>,
+    finputs: set<NP>,
+    foutputs: set<NP>,
+    f: map<NP, bool> --> map<NP, bool>
+  )
+
+  opaque predicate EntitySomewhatValid(c: Circuit, e: Entity)
+    requires CircuitValid(c)
+  {
+    && ScValid(c, e.sc)
+    && (AllPossibleOutputs(c, e.sc) >= e.foutputs >= AllOutputs(c, e.sc))
+    && (e.finputs == AllInputs(c, e.sc))
+  }
+
+  lemma EntityFInputsAreValid(c: Circuit, e: Entity)
+    requires CircuitValid(c)
+    requires EntitySomewhatValid(c, e)
+    ensures forall np :: np in e.finputs ==> NPValid(c, np)
+  {
+    reveal ScValid();
+    reveal EntitySomewhatValid();
+    reveal NPsValid();
+  }
+
+  lemma EntityFOutputsAreValid(c: Circuit, e: Entity)
+    requires CircuitValid(c)
+    requires EntitySomewhatValid(c, e)
+    ensures forall np :: np in e.foutputs ==> NPValid(c, np)
+  {
+    reveal ScValid();
+    reveal EntitySomewhatValid();
+    reveal NPsValid();
+  }
+
+  ghost opaque predicate EntityFValid(c: Circuit, e: Entity)
+  {
+    forall knowns: map<NP, bool> :: knowns.Keys == e.finputs ==>
+      && e.f.requires(knowns)
+      && (e.f(knowns).Keys == e.foutputs)
+  }
+
+  ghost opaque predicate EntityEvaluatesCorrectly(c: Circuit, e: Entity)
+    requires CircuitValid(c)
+    requires ScValid(c, e.sc)
+    requires EntityFValid(c, e)
+    requires EntitySomewhatValid(c, e)
+  {
+    reveal ScValid();
+    EntityFOutputsAreValid(c, e);
+    reveal EntityFValid();
+    forall knowns: map<NP, bool> :: knowns.Keys == e.finputs ==>
+      forall np :: np in e.foutputs ==>
+        && Evaluate(c, np, knowns) == EvalOk(e.f(knowns)[np])
+  }
+
+  ghost predicate EntityValid(c: Circuit, e: Entity)
+    requires CircuitValid(c)
+  {
+    && EntitySomewhatValid(c, e)
+    && EntityFValid(c, e)
+    && ScValid(c, e.sc)
+    && EntityEvaluatesCorrectly(c, e)
+  }
+
+  lemma FInputsInSc(c: Circuit, e: Entity)
+    requires CircuitValid(c)
+    requires EntitySomewhatValid(c, e)
+    ensures NPsInSc(e.sc, e.finputs)
+  {
+    reveal EntitySomewhatValid();
+    reveal NPsInSc();
+  }
+
+  lemma FOutputsInSc(c: Circuit, e: Entity)
+    requires CircuitValid(c)
+    requires EntitySomewhatValid(c, e)
+    ensures NPsInSc(e.sc, e.foutputs)
+  {
+    reveal NPsInSc();
+    reveal EntitySomewhatValid();
+    assert AllPossibleOutputs(c, e.sc) >= e.foutputs;
+  }
+
+  lemma StaysInSc(c: Circuit, e: Entity, np: NP)
+    requires CircuitValid(c)
+    requires EntitySomewhatValid(c, e)
+    requires INPValid(c, np)
+    requires np.n in e.sc
+    requires np !in e.finputs
+    ensures np in c.PortSource
+    ensures c.PortSource[np].n in e.sc
+  {
+    reveal CircuitValid();
+    reveal EntitySomewhatValid();
+    reveal UnconnInputs();
+    reveal ConnInputs();
+  }
+
+  predicate OutputsInFOutputs(c: Circuit, e: Entity)
+    requires CircuitValid(c)
+    requires ScValid(c, e.sc)
+  {
+    e.foutputs >= ConnOutputs(c, e.sc)
+  }
+
+  function SwapEntityF(c: Circuit, e: Entity, f: map<NP, bool> --> map<NP, bool>): (r: Entity)
+    requires EntityValid(c, e)
+    requires MapFunctionValid(MapFunction(e.finputs, e.foutputs, f))
+    ensures EntityValid(c, r)
+  {
+    reveal EntitySomewhatValid();
+    reveal EntityFValid();
+    reveal ScValid();
+    reveal EntityEvaluatesCorrectly();
+    Entity(e.sc, e.finputs, e.foutputs, f)
+  }
+
+  lemma NPInFInputsOfIslandNotInPortSource(c: Circuit, e: Entity, np: NP) 
+    requires CircuitValid(c)
+    requires IsIsland(c, e.sc)
+    requires EntityValid(c, e)
+    requires np in e.finputs
+    ensures np !in c.PortSource
+  {
+    assert np in AllInputs(c, e.sc) by {
+      reveal EntitySomewhatValid();
+    }
+    assert |ConnInputs(c, e.sc)| == 0 by {
+      IsIslandNoInputs(c, e.sc);
+    }
+    assert np in UnconnInputs(c, e.sc) || np in FinalInputs(c, e.sc) || np in SeqInputs(c, e.sc);
+    if np in UnconnInputs(c, e.sc) {
+      assert np !in c.PortSource by {
+        reveal UnconnInputs();
+      }
+    }
+    if np in FinalInputs(c, e.sc) {
+      assert ONPValid(c, np) by {
+        reveal FinalInputs();
+      }
+    }
+    if np in SeqInputs(c, e.sc) {
+      assert ONPValid(c, np) by {
+        reveal SeqInputs();
+      }
+    }
+  }
+
+}
