Attempt2/IslandBundle.dfy
@@ -1,0 +1,198 @@
+module IslandBundle {
+
+  import opened Std.Wrappers
+
+  import opened Circ
+  import opened Entity
+  import opened ConservedSubcircuit
+  import opened Utils
+  import opened Connection
+  import opened ConnectionEval
+  import opened Subcircuit
+
+  // All nodes in the circuit are in exactly one Equiv.
+  // This helps with reasoning about the circuit when adding stuff.
+
+  datatype IslandBundle = IslandBundle(
+    c: Circuit,
+    es: seq<Option<Entity>>,
+    NodeEquiv: map<CNode, nat>
+  )
+
+  ghost opaque predicate IslandBundleValid(eb: IslandBundle) {
+    && CircuitValid(eb.c)
+    && (forall e :: e in eb.es && e.Some? ==> EntityValid(eb.c, e.value))
+    // All Equivs are islands (i.e. not connections in or out)
+    && (forall e :: e in eb.es && e.Some? ==> IsIsland(eb.c, e.value.sc))
+    // NodeEquiv points to an Equiv in the eb.es seq.
+    && (forall n :: n in eb.NodeEquiv ==> eb.NodeEquiv[n] < |eb.es|)
+    // All nodes in an Equiv must be pointed to from this NodeEquiv map
+    && (forall index: nat :: index < |eb.es| && eb.es[index].Some? ==>
+        (forall n :: n in eb.es[index].value.sc ==> n in eb.NodeEquiv && eb.NodeEquiv[n] == index))
+  }
+
+  lemma IslandBundleToSetsNoIntersection(eb: IslandBundle, e1_index: nat, e2_index: nat)
+    requires IslandBundleValid(eb)
+    requires e1_index != e2_index
+    requires e1_index < |eb.es| && eb.es[e1_index].Some?
+    requires e2_index < |eb.es| && eb.es[e2_index].Some?
+    ensures
+      var e1 := eb.es[e1_index].value;
+      var e2 := eb.es[e2_index].value;
+      SetsNoIntersection(e1.sc, e2.sc)
+  {
+    reveal IslandBundleValid();
+  }
+
+  lemma IsIslandToNoScOutputs(c: Circuit, sc: set<CNode>)
+    requires CircuitValid(c)
+    requires IsIsland(c, sc)
+    ensures ScOutputBoundary(c, sc) == {}
+  {
+    reveal CircuitValid();
+    reveal IsIsland();
+  }
+
+  lemma AddEntityCorrect(eb: IslandBundle, new_c: Circuit, new_e: Entity)
+    requires IslandBundleValid(eb)
+    requires CircuitConserved(eb.c, new_c)
+    requires CircuitUnconnected(eb.c, new_c)
+    requires CircuitValid(new_c)
+    requires EntityValid(new_c, new_e)
+    requires IsIsland(new_c, new_e.sc)
+    requires forall n :: n in new_e.sc ==> n !in eb.NodeEquiv
+    requires new_c.NodeKind.Keys == eb.c.NodeKind.Keys + new_e.sc
+    ensures IslandBundleValid(AddEntityImpl(eb, new_c, new_e).0)
+  {
+    var (new_eb, ref) := AddEntityImpl(eb, new_c, new_e);
+    assert CircuitValid(eb.c) && CircuitValid(new_eb.c) by {
+      reveal IslandBundleValid();
+    }
+    forall index: nat | index < |eb.es| && eb.es[index].Some?
+      ensures
+        var e := eb.es[index].value;
+        && EntityValid(new_c, e)
+        && IsIsland(new_c, e.sc)
+    {
+      var e := eb.es[index].value;
+      assert IsIsland(eb.c, e.sc) by {
+        reveal IslandBundleValid();
+      }
+      assert EntityValid(eb.c, e) by {
+        reveal IslandBundleValid();
+      }
+      assert ScValid(eb.c, e.sc) by {
+      }
+      assert ScValid(new_c, e.sc) by {
+        reveal ScValid();
+      }
+      IsIslandConserved(eb.c, new_eb.c, e.sc);
+      IsIslandToNoScOutputs(eb.c, e.sc);
+      IsIslandToNoScOutputs(new_eb.c, e.sc);
+      CircuitConservedToSubcircuitConserved(eb.c, new_eb.c, e.sc);
+      assert SubcircuitConserved(eb.c, new_eb.c, e.sc);
+      assert OutputsInFOutputs(new_eb.c, e) by {
+        IsIslandNoOutputs(new_eb.c, e.sc);
+        reveal IsIsland();
+        reveal ConnOutputs();
+        assert IsIsland(new_eb.c, e.sc);
+        assert |ConnOutputs(new_eb.c, e.sc)| == 0;
+      }
+      EntityConserved(eb.c, new_eb.c, e);
+      assert EntityValid(new_eb.c, e) by {
+        reveal IslandBundleValid();
+      }
+    }
+    assert IslandBundleValid(new_eb) by {
+      reveal IslandBundleValid();
+    }
+  }
+
+  function AddEntityImpl(eb: IslandBundle, new_c: Circuit, new_e: Entity): (r: (IslandBundle, nat))
+    requires IslandBundleValid(eb)
+    requires CircuitConserved(eb.c, new_c)
+    requires CircuitUnconnected(eb.c, new_c)
+    requires CircuitValid(new_c)
+    requires EntityValid(new_c, new_e)
+    requires IsIsland(new_c, new_e.sc)
+    requires forall n :: n in new_e.sc ==> n !in eb.NodeEquiv
+    requires new_c.NodeKind.Keys == eb.c.NodeKind.Keys + new_e.sc
+    ensures r.1 < |r.0.es|
+    ensures r.0.es[r.1].Some?
+    ensures r.0.es[r.1].value == new_e
+  {
+    var new_node_equiv := (map n | n in new_e.sc :: n := |eb.es|);
+    var new_eb := IslandBundle(
+      new_c,
+      eb.es + [Some(new_e)],
+      AddMaps(eb.NodeEquiv, new_node_equiv)
+    );
+    (new_eb, |eb.es|)
+  }
+
+  function AddEntity(eb: IslandBundle, new_c: Circuit, new_e: Entity): (r: (IslandBundle, nat))
+    requires IslandBundleValid(eb)
+    requires CircuitConserved(eb.c, new_c)
+    requires CircuitUnconnected(eb.c, new_c)
+    requires CircuitValid(new_c)
+    requires EntityValid(new_c, new_e)
+    requires IsIsland(new_c, new_e.sc)
+    requires forall n :: n in new_e.sc ==> n !in eb.NodeEquiv
+    requires new_c.NodeKind.Keys == eb.c.NodeKind.Keys + new_e.sc
+    ensures IslandBundleValid(r.0)
+    ensures r.1 < |r.0.es|
+    ensures r.0.es[r.1].Some?
+    ensures r.0.es[r.1].value == new_e
+  {
+    AddEntityCorrect(eb, new_c, new_e);
+    AddEntityImpl(eb, new_c, new_e)
+  }
+
+  function ComposeEquivsImpl(
+      eb: IslandBundle, new_c: Circuit, e1_index: nat, e2_index: nat,
+      connection: map<NP, NP>): (r: IslandBundle)
+    requires IslandBundleValid(eb)
+    requires CircuitConserved(eb.c, new_c)
+    requires CircuitUnconnected(eb.c, new_c)
+    requires CircuitValid(new_c)
+    requires e1_index != e2_index
+    requires e1_index < |eb.es| && eb.es[e1_index].Some?
+    requires e2_index < |eb.es| && eb.es[e2_index].Some?
+    requires ScValid(eb.c, eb.es[e1_index].value.sc)
+    requires ScValid(eb.c, eb.es[e2_index].value.sc)
+    requires ConnectionValid(eb.c, eb.es[e1_index].value, eb.es[e2_index].value, connection)
+  {
+    assert CircuitValid(eb.c) by {
+      reveal IslandBundleValid();
+    }
+    var e1 := eb.es[e1_index].value;
+    var e2 := eb.es[e2_index].value;
+    assert SetsNoIntersection(e1.sc, e2.sc) by {
+      IslandBundleToSetsNoIntersection(eb, e1_index, e2_index);
+    }
+    assert ScValid(eb.c, e1.sc) &&  ScValid(eb.c, e2.sc) by {
+      reveal IslandBundleValid();
+      reveal ScValid();
+    }
+    assert EntityValid(eb.c, e1) && EntityValid(eb.c, e2) by {
+      reveal IslandBundleValid();
+    }
+
+
+    assert IsIsland(eb.c, e2.sc) && IsIsland(eb.c, e1.sc) by {
+      reveal IslandBundleValid();
+    }
+    var (new_c, new_e) := ConnectEntities(eb.c, e1, e2, connection);
+    var new_es := seq(|eb.es|, (index: nat) requires index < |eb.es| => (
+      if (index == e1_index || index == e2_index) then None else eb.es[index])) + [Some(new_e)];
+    var new_index := |new_es|-1;
+    var new_node_equiv := (map key | key in eb.NodeEquiv.Keys :: if key in new_e.sc then new_index else eb.NodeEquiv[key]);
+    var new_eb := IslandBundle(
+      new_c,
+      new_es,
+      new_node_equiv
+    );
+    new_eb
+  }
+
+}
