Attempt2/Subcircuit.dfy
@@ -1,0 +1,360 @@
+module Subcircuit {
+
+  import opened Circ
+  import opened Utils
+
+  opaque predicate NPsInSc(sc: set<CNode>, nps: set<NP>)
+  {
+    forall np :: np in nps ==> np.n in sc
+  }
+
+  opaque predicate NPsValid(c: Circuit, nps: set<NP>)
+  {
+    forall np :: np in nps ==> NPValid(c, np)
+  }
+
+  opaque predicate INPsValid(c: Circuit, nps: set<NP>)
+  {
+    forall np :: np in nps ==> INPValid(c, np)
+  }
+
+  opaque predicate ONPsValid(c: Circuit, nps: set<NP>)
+  {
+    forall np :: np in nps ==> ONPValid(c, np)
+  }
+
+  lemma INPsAndONPsNoIntersection(c: Circuit, inps: set<NP>, onps: set<NP>)
+    requires INPsValid(c, inps)
+    requires ONPsValid(c, onps)
+    ensures SetsNoIntersection(inps, onps)
+  {
+    reveal INPsValid();
+    reveal ONPsValid();
+  }
+
+  opaque function ConnInputs(c: Circuit, sc: set<CNode>): (r: set<NP>)
+    requires CircuitValid(c)
+    requires ScValid(c, sc)
+    ensures NPsInSc(sc, r)
+    ensures INPsValid(c, r)
+  {
+    reveal CircuitValid();
+    reveal NPsInSc();
+    reveal INPsValid();
+    (set np: NP | np.n in sc && np in c.PortSource && c.PortSource[np].n !in sc :: np)
+  }
+
+  opaque function UnconnInputs(c: Circuit, sc: set<CNode>): (r: set<NP>)
+    requires CircuitValid(c)
+    requires ScValid(c, sc)
+    ensures NPsInSc(sc, r)
+    ensures INPsValid(c, r)
+  {
+    reveal NPsInSc();
+    reveal ScValid();
+    reveal INPsValid();
+    (set np: NP | np in AllNPFromNodes(c, sc) && INPValid(c, np) && np !in c.PortSource :: np)
+  }
+
+  lemma UnconnInputsAdd(c: Circuit, sc1: set<CNode>, sc2: set<CNode>)
+    requires CircuitValid(c)
+    requires ScValid(c, sc1)
+    requires ScValid(c, sc2)
+    ensures ScValid(c, sc1 + sc2)
+    ensures UnconnInputs(c, sc1) + UnconnInputs(c, sc2) == UnconnInputs(c, sc1 + sc2)
+  {
+    reveal ScValid();
+    reveal UnconnInputs();
+  }
+
+  opaque function ConnOutputs(c: Circuit, sc: set<CNode>): (r: set<NP>)
+    requires CircuitValid(c)
+    requires ScValid(c, sc)
+    ensures NPsInSc(sc, r)
+    ensures ONPsValid(c, r)
+  {
+    reveal NPsInSc();
+    reveal ONPsValid();
+    reveal CircuitValid();
+    (set np: NP | np.n !in sc && np in c.PortSource && c.PortSource[np].n in sc ::
+      c.PortSource[np])
+  }
+
+  opaque function SeqInputs(c: Circuit, sc: set<CNode>): (r: set<NP>)
+    requires ScValid(c, sc)
+    ensures NPsInSc(sc, r)
+    ensures ONPsValid(c, r)
+  {
+    reveal NPsInSc();
+    reveal ScValid();
+    reveal ONPsValid();
+    (set n | (n in sc) && c.NodeKind[n].CSeq? :: NP(n, OUTPUT_0))
+  }
+
+  opaque function SeqOutputs(c: Circuit, sc: set<CNode>): (r: set<NP>)
+    requires ScValid(c, sc)
+    ensures NPsInSc(sc, r)
+    ensures INPsValid(c, r)
+  {
+    reveal NPsInSc();
+    reveal ScValid();
+    reveal INPsValid();
+    (set n | (n in sc) && c.NodeKind[n].CSeq? :: NP(n, INPUT_0))
+  }
+
+  opaque function FinalInputs(c: Circuit, sc: set<CNode>): (r: set<NP>)
+    requires ScValid(c, sc)
+    ensures NPsInSc(sc, r)
+    ensures ONPsValid(c, r)
+  {
+    reveal NPsInSc();
+    reveal ScValid();
+    reveal ONPsValid();
+    (set n | (n in sc) && c.NodeKind[n].CInput? :: NP(n, OUTPUT_0))
+  }
+
+  opaque function FinalOutputs(c: Circuit, sc: set<CNode>): (r: set<NP>)
+    requires ScValid(c, sc)
+    ensures NPsInSc(sc, r)
+    ensures INPsValid(c, r)
+  {
+    reveal NPsInSc();
+    reveal ScValid();
+    reveal INPsValid();
+    (set n | (n in sc) && c.NodeKind[n].COutput? :: NP(n, INPUT_0))
+  }
+
+  opaque function AllINPs(c: Circuit, sc: set<CNode>): (r: set<NP>)
+    requires ScValid(c, sc)
+    ensures NPsInSc(sc, r)
+    ensures INPsValid(c, r)
+  {
+    reveal NPsInSc();
+    reveal ScValid();
+    reveal INPsValid();
+    (set np | np in AllNPFromNodes(c, sc) && INPValid(c, np) :: np)
+  }
+
+  opaque function AllONPs(c: Circuit, sc: set<CNode>): (r: set<NP>)
+    requires ScValid(c, sc)
+    ensures NPsInSc(sc, r)
+    ensures ONPsValid(c, r)
+  {
+    reveal NPsInSc();
+    reveal ScValid();
+    reveal ONPsValid();
+    (set np | np in AllNPFromNodes(c, sc) && ONPValid(c, np) :: np)
+  }
+  
+  function AllPossibleOutputs(c: Circuit, sc: set<CNode>): (r: set<NP>)
+    requires ScValid(c, sc)
+    ensures NPsInSc(sc, r)
+    ensures NPsValid(c, r)
+  {
+    reveal NPsInSc();
+    reveal ScValid();
+    reveal NPsValid();
+    reveal INPsValid();
+    reveal ONPsValid();
+    AllONPs(c, sc) + SeqOutputs(c, sc) + FinalOutputs(c, sc)
+  }
+
+  function AllInputs(c: Circuit, sc: set<CNode>): (r: set<NP>)
+    requires CircuitValid(c)
+    requires ScValid(c, sc)
+    ensures NPsInSc(sc, r)
+    ensures NPsValid(c, r)
+  {
+    reveal NPsInSc();
+    reveal ScValid();
+    reveal NPsValid();
+    reveal INPsValid();
+    reveal ONPsValid();
+    UnconnInputs(c, sc) + ConnInputs(c, sc) + SeqInputs(c, sc) + FinalInputs(c, sc)
+  }
+  
+  function AllOutputs(c: Circuit, sc: set<CNode>): (r: set<NP>)
+    requires CircuitValid(c)
+    requires ScValid(c, sc)
+    ensures NPsInSc(sc, r)
+    ensures NPsValid(c, r)
+  {
+    reveal NPsInSc();
+    reveal ScValid();
+    reveal NPsValid();
+    reveal INPsValid();
+    reveal ONPsValid();
+    ConnOutputs(c, sc) + SeqOutputs(c, sc) + FinalOutputs(c, sc)
+  }
+
+  function ConnFromTo(c: Circuit, sca: set<CNode>, scb: set<CNode>): (r: set<NP>)
+    requires CircuitValid(c)
+    requires ScValid(c, sca)
+    requires ScValid(c, scb)
+    ensures NPsInSc(scb, r)
+  {
+    reveal NPsInSc();
+    reveal ScValid();
+    (set np: NP | (np.n in scb) && (np in c.PortSource) && (c.PortSource[np].n in sca) :: np)
+  }
+
+  opaque predicate NoConnFromTo(c: Circuit, sca: set<CNode>, scb: set<CNode>)
+    requires CircuitValid(c)
+    requires ScValid(c, sca)
+    requires ScValid(c, scb)
+  {
+    |ConnFromTo(c, sca, scb)| == 0
+  }
+
+  function Complement(c: Circuit, sc: set<CNode>): set<CNode>
+  {
+    c.NodeKind.Keys - sc
+  }
+
+  lemma InScOrComplement(c: Circuit, sc: set<CNode>, n: CNode)
+    requires CircuitValid(c)
+    requires ScValid(c, sc)
+    requires NodeValid(c, n)
+    ensures
+      var sccomp := SubcircuitComplement(c, sc);
+      ((n in sc) || (n in sccomp)) &&
+      !((n in sc) && (n in sccomp))
+  {
+    var sccomp := SubcircuitComplement(c, sc);
+    reveal CircuitValid();
+    reveal ScValid();
+    assert (n in sc) || (n in sccomp);
+    assert !((n in sc) && (n in sccomp));
+  }
+
+  opaque ghost predicate IsIsland(c: Circuit, sc: set<CNode>)
+  {
+    && (forall np :: np in c.PortSource && np.n in sc ==> c.PortSource[np].n in sc)
+    && (forall np :: np in c.PortSource && np.n !in sc ==> c.PortSource[np].n !in sc)
+  }
+
+  lemma IsIslandNoConns(c: Circuit, sc1: set<CNode>, sc2: set<CNode>)
+    requires CircuitValid(c)
+    requires ScValid(c, sc1)
+    requires ScValid(c, sc2)
+    requires SetsNoIntersection(sc1, sc2)
+    requires IsIsland(c, sc1)
+    ensures NoConnFromTo(c, sc1, sc2) && NoConnFromTo(c, sc2, sc1)
+  {
+    reveal CircuitValid();
+    reveal ScValid();
+    reveal IsIsland();
+    reveal NoConnFromTo();
+    if |ConnFromTo(c, sc1, sc2)| > 0 {
+      var np :| np in ConnFromTo(c, sc1, sc2);
+      assert np.n in sc2 && np in c.PortSource && c.PortSource[np].n in sc1;
+      NotInBoth(np.n, sc1, sc2);
+      assert false;
+    }
+    if |ConnFromTo(c, sc2, sc1)| > 0 {
+      var np :| np in ConnFromTo(c, sc2, sc1);
+      assert np.n in sc1 && np in c.PortSource && c.PortSource[np].n in sc2;
+      NotInBoth(c.PortSource[np].n, sc1, sc2);
+      assert np.n in sc1 && np in c.PortSource && c.PortSource[np].n !in sc1;
+      assert false;
+    }
+  }
+
+  lemma NoConnsToComplementIsIsland(c: Circuit, sc: set<CNode>)
+    requires CircuitValid(c)
+    requires ScValid(c, sc)
+    requires
+      var sccomp := SubcircuitComplement(c, sc);
+      NoConnFromTo(c, sc, sccomp) && NoConnFromTo(c, sccomp, sc)
+    ensures
+      IsIsland(c, sc)
+  {
+    reveal CircuitValid();
+    reveal ScValid();
+    reveal NoConnFromTo();
+    reveal IsIsland();
+    var sccomp := SubcircuitComplement(c, sc);
+    assert |ConnFromTo(c, sc, sccomp)| == 0;
+    assert |ConnFromTo(c, sccomp, sc)| == 0;
+    forall np: NP | np in c.PortSource
+      ensures np.n in sc ==> c.PortSource[np].n in sc
+      ensures np.n !in sc ==> c.PortSource[np].n !in sc
+    {
+      InScOrComplement(c, sc, np.n);
+      assert ONPValid(c, c.PortSource[np]);
+      InScOrComplement(c, sc, c.PortSource[np].n);
+
+      if (np.n in sccomp) && (c.PortSource[np].n in sc) {
+        assert np in ConnFromTo(c, sc, sccomp);
+      }
+      assert !((np.n in sccomp) && (c.PortSource[np].n in sc));
+      if (np.n in sc) && (c.PortSource[np].n in sccomp) {
+        assert np in ConnFromTo(c, sccomp, sc);
+      }
+      assert !((np.n in sc) && (c.PortSource[np].n in sccomp));
+
+      if np.n in sc {
+        assert c.PortSource[np].n in sc;
+      } else {
+        assert c.PortSource[np].n !in sc;
+      }
+    }
+  }
+
+  lemma SubcircuitComplementOwnInverse(c: Circuit, sc: set<CNode>)
+    requires CircuitValid(c)
+    requires ScValid(c, sc)
+    ensures SubcircuitComplement(c, SubcircuitComplement(c, sc)) == sc
+  {
+    reveal CircuitValid();
+    reveal ScValid();
+  }
+
+
+  lemma IsIslandComplementIsIsland(c: Circuit, sc: set<CNode>)
+    requires CircuitValid(c)
+    requires ScValid(c, sc)
+    requires IsIsland(c, sc)
+    ensures IsIsland(c, SubcircuitComplement(c, sc))
+  {
+    reveal IsIsland();
+    reveal CircuitValid();
+    reveal ScValid();
+    var sccomp := SubcircuitComplement(c, sc);
+    IsIslandNoConns(c, sc, sccomp);
+    assert NoConnFromTo(c, sc, sccomp);
+    assert NoConnFromTo(c, sccomp, sc);
+    SubcircuitComplementOwnInverse(c, sc);
+    assert sc == SubcircuitComplement(c, sccomp);
+    NoConnsToComplementIsIsland(c, sccomp);
+  }
+
+  lemma IsIslandNoOutputs(c: Circuit, sc: set<CNode>)
+    requires CircuitValid(c)
+    requires ScValid(c, sc)
+    requires IsIsland(c, sc)
+    ensures |ConnOutputs(c, sc)| == 0
+  {
+    reveal CircuitValid();
+    reveal ScValid();
+    reveal IsIsland();
+    reveal ConnOutputs();
+  }
+
+  lemma IsIslandNoInputs(c: Circuit, sc: set<CNode>)
+    requires CircuitValid(c)
+    requires ScValid(c, sc)
+    requires IsIsland(c, sc)
+    ensures |ConnInputs(c, sc)| == 0
+  {
+    reveal CircuitValid();
+    reveal ScValid();
+    reveal IsIsland();
+    reveal ConnInputs();
+  }
+
+  opaque predicate PathInSubcircuit(path: seq<NP>, sc: set<CNode>)
+  {
+    forall np :: np in path ==> np.n in sc
+  }
+}
